verif/btrees/verif_isempty.v
@@ -1,0 +1,56 @@
+(** * verif_isvalid.v : Correctness proof of isValid, isFirst and RL_CursorIsValid *)
+
+Require Import VST.floyd.proofauto.
+Require Import VST.floyd.library.
+Require Import relation_mem.
+Instance CompSpecs : compspecs. make_compspecs prog. Defined.
+Definition Vprog : varspecs. mk_varspecs prog. Defined.
+
+Require Import VST.msl.wand_frame.
+Require Import VST.msl.iter_sepcon.
+Require Import VST.floyd.reassoc_seq.
+Require Import VST.floyd.field_at_wand.
+Require Import FunInd.
+Require Import btrees.
+Require Import btrees_sep.
+Require Import btrees_spec.
+Require Import index.
+
+Lemma body_isempty : semax_body Vprog Gprog f_RL_IsEmpty RL_IsEmpty_spec.
+Proof.
+  start_function. 
+  forward_if (PROP ( cursor <> nullval )
+                   LOCAL (gvars gv; temp _cursor cursor)
+                   SEP (mem_mgr gv; relation_rep r (get_numrec r); cursor_rep c r cursor)).
+  + forward. entailer.
+  + subst cursor.
+    unfold cursor_rep. assert_PROP False.
+  - Intros a b. destruct r. rewrite data_at_isptr. entailer.
+  - contradiction.
+    + unfold cursor_rep. destruct r. Intros anc_end idx_end. forward.
+      unfold relation_rep. Intros. forward.
+      destruct n. simpl getval. unfold btnode_rep; fold btnode_rep; fold le_iter_sepcon.
+      Intros ent_end.
+      forward.
+      Intros. forward_if.
+      forward. entailer!. simpl numKeys.
+      replace (numKeys_le l) with 0%nat.
+      * easy.
+      * apply Nat2Z.inj, repr_inj_unsigned.
+        easy. split. omega. 
+        transitivity (Z.of_nat Fanout).
+        -- apply inj_le. replace (numKeys_le l) with (numKeys (btnode val o l b b0 b1 v0)) by reflexivity.
+           apply H. apply sub_refl.
+        -- easy.
+        -- easy.
+      * unfold relation_rep, cursor_rep; entailer!. (* This proof is not so pretty. *)
+        Exists anc_end. entailer. Exists idx_end. entailer.
+        unfold btnode_rep. fold btnode_rep. fold le_iter_sepcon. Exists ent_end. entailer!.
+      * forward. entailer!. simpl. 
+        destruct (nat_eq_dec (numKeys_le l) 0%nat). 
+        destruct l. simpl in H1. contradiction. inversion e. reflexivity.
+        unfold cursor_rep, relation_rep. entailer!.
+        Exists anc_end. entailer!. Exists idx_end. entailer!.
+        unfold btnode_rep. fold btnode_rep. fold le_iter_sepcon.
+        Exists ent_end. entailer!.
+Qed.
